Move LTL_Stutter to Stuttering_Equivalence
Cleand up and updated notation in Stuttering_Equivalence

thys/Stuttering_Equivalence/PLTL.thy
@@ -2,22 +2,14 @@ theory PLTL
   imports Main LTL.LTL Samplers StutterEquivalence
 begin
 
-section \<open>Stuttering Invariant PLTL Formulas\<close>
+section \<open>Stuttering Invariant LTL Formulas\<close>
 
 text \<open>
-  We define the syntax and semantics of propositional linear-time
-  temporal logic PLTL and show that its next-free fragment is
-  invariant to finite stuttering.
+  We show that the next-free fragment of propositional linear-time
+  temporal logic PLTL is invariant to finite stuttering.
 \<close>
 
-notation False_ltlp ("false")
-  and Implies_ltlp ("implies")
-  and Atom_ltlp ("atom")
-  and Until_ltlp ("until")
-  and Next_ltlp ("next")
-  and atoms_pltl ("atoms")
-
-subsection \<open>Finite Conjunctions and Disjunctions\<close>
+subsection \<open>Finite Conjunctions and Disjunctions in PLTL\<close>
 
 (* It would be tempting to define these operators as follows:
 
@@ -194,44 +186,44 @@ text \<open>
 theorem next_free_stutter_invariant:
   "next_free \<phi> \<Longrightarrow> stutter_invariant (\<phi>::'a pltl)"
 proof (induct "\<phi>")
-    show "stutter_invariant false" by auto
+    show "stutter_invariant false\<^sub>p" by auto
 next
   fix p :: "'a \<Rightarrow> bool"
-  show "stutter_invariant (atom p)"
+  show "stutter_invariant (atom\<^sub>p(p))"
   proof
     fix \<sigma> \<tau>
-    assume "\<sigma> \<approx> \<tau>" "\<sigma> \<Turnstile>\<^sub>p atom p"
-    thus "\<tau> \<Turnstile>\<^sub>p atom p" by (simp add: stutter_equiv_0)
+    assume "\<sigma> \<approx> \<tau>" "\<sigma> \<Turnstile>\<^sub>p atom\<^sub>p(p)"
+    thus "\<tau> \<Turnstile>\<^sub>p atom\<^sub>p(p)" by (simp add: stutter_equiv_0)
   qed
 next
   fix \<phi> \<psi> :: "'a pltl"
   assume ih: "next_free \<phi> \<Longrightarrow> stutter_invariant \<phi>"
              "next_free \<psi> \<Longrightarrow> stutter_invariant \<psi>"
-  assume "next_free (implies \<phi> \<psi>)"
-  with ih show "stutter_invariant (implies \<phi> \<psi>)" by auto
+  assume "next_free (\<phi> implies\<^sub>p \<psi>)"
+  with ih show "stutter_invariant (\<phi> implies\<^sub>p \<psi>)" by auto
 next
   fix \<phi> :: "'a pltl"
-  assume "next_free (next \<phi>)"  \<comment> \<open>hence contradiction\<close>
-  thus "stutter_invariant (next \<phi>)" by simp
+  assume "next_free (X\<^sub>p \<phi>)"  \<comment> \<open>hence contradiction\<close>
+  thus "stutter_invariant (X\<^sub>p \<phi>)" by simp
 next
   fix \<phi> \<psi> :: "'a pltl"
   assume ih: "next_free \<phi> \<Longrightarrow> stutter_invariant \<phi>"
              "next_free \<psi> \<Longrightarrow> stutter_invariant \<psi>"
-  assume "next_free (until \<phi> \<psi>)"
+  assume "next_free (\<phi> U\<^sub>p \<psi>)"
   with ih have stinv: "stutter_invariant \<phi>" "stutter_invariant \<psi>" by auto
-  show "stutter_invariant (until \<phi> \<psi>)"
+  show "stutter_invariant (\<phi> U\<^sub>p \<psi>)"
   proof
     fix \<sigma> \<tau>
-    assume st: "\<sigma> \<approx> \<tau>" and unt: "\<sigma> \<Turnstile>\<^sub>p until \<phi> \<psi>"
+    assume st: "\<sigma> \<approx> \<tau>" and unt: "\<sigma> \<Turnstile>\<^sub>p \<phi> U\<^sub>p \<psi>"
     from unt obtain m
-      where 1: "\<sigma>[m..] \<Turnstile>\<^sub>p \<psi>" and 2: "\<forall>j<m. \<sigma>[j..] \<Turnstile>\<^sub>p \<phi>" by auto
+      where 1: "\<sigma>[m..] \<Turnstile>\<^sub>p \<psi>" and 2: "\<forall>j<m. (\<sigma>[j..] \<Turnstile>\<^sub>p \<phi>)" by auto
     from st obtain n
-      where 3: "\<sigma>[m..] \<approx> \<tau>[n..]" and 4: "\<forall>i<n. \<exists>j<m. \<sigma>[j..] \<approx> \<tau>[i..]"
+      where 3: "(\<sigma>[m..]) \<approx> (\<tau>[n..])" and 4: "\<forall>i<n. \<exists>j<m. (\<sigma>[j..]) \<approx> (\<tau>[i..])"
       by (rule stutter_equiv_suffixes_right)
     from 1 3 stinv have "\<tau>[n..] \<Turnstile>\<^sub>p \<psi>" by auto
     moreover
-    from 2 4 stinv have "\<forall>i<n. \<tau>[i..] \<Turnstile>\<^sub>p \<phi>" by force
-    ultimately show "\<tau> \<Turnstile>\<^sub>p until \<phi> \<psi>" by auto
+    from 2 4 stinv have "\<forall>i<n. (\<tau>[i..] \<Turnstile>\<^sub>p \<phi>)" by force
+    ultimately show "\<tau> \<Turnstile>\<^sub>p \<phi> U\<^sub>p \<psi>" by auto
   qed
 qed
 
@@ -251,27 +243,27 @@ text \<open>
 \<close>
 
 
-lemma atoms_OR [simp]: 
+lemma atoms_pltl_OR [simp]:
   assumes fin: "finite (\<Phi>::'a pltl set)"
-  shows "atoms (OR \<Phi>) = (\<Union>\<phi>\<in>\<Phi>. atoms \<phi>)"
+  shows "atoms_pltl (OR \<Phi>) = (\<Union>\<phi>\<in>\<Phi>. atoms_pltl \<phi>)"
 proof -
   {
     fix \<psi>::"'a pltl"
     assume "fold_graph Or_ltlp False_ltlp \<Phi> \<psi>"
-    hence "atoms \<psi> = (\<Union>\<phi>\<in>\<Phi>. atoms \<phi>)"
+    hence "atoms_pltl \<psi> = (\<Union>\<phi>\<in>\<Phi>. atoms_pltl \<phi>)"
       by (rule fold_graph.induct) auto
   }
   with fold_graph_OR[OF fin] show ?thesis by simp
 qed
 
-lemma atoms_AND [simp]: 
+lemma atoms_pltl_AND [simp]:
   assumes fin: "finite (\<Phi>::'a pltl set)"
-  shows "atoms (AND \<Phi>) = (\<Union>\<phi>\<in>\<Phi>. atoms \<phi>)"
+  shows "atoms_pltl (AND \<Phi>) = (\<Union>\<phi>\<in>\<Phi>. atoms_pltl \<phi>)"
 proof -
   {
     fix \<psi>::"'a pltl"
     assume "fold_graph And_ltlp True_ltlp \<Phi> \<psi>"
-    hence "atoms \<psi> = (\<Union>\<phi>\<in>\<Phi>. atoms \<phi>)"
+    hence "atoms_pltl \<psi> = (\<Union>\<phi>\<in>\<Phi>. atoms_pltl \<phi>)"
       by (rule fold_graph.induct) auto
   }
   with fold_graph_AND[OF fin] show ?thesis by simp
@@ -331,40 +323,40 @@ text \<open>
   evaluate that formula to the same value.  
 \<close>
 
-lemma pltl_seq_sim: "\<sigma> \<simeq>(atoms \<phi>)\<simeq> \<tau> \<Longrightarrow> (\<sigma> \<Turnstile>\<^sub>p \<phi>) = (\<tau> \<Turnstile>\<^sub>p \<phi>)"
+lemma pltl_seq_sim: "\<sigma> \<simeq> atoms_pltl \<phi> \<simeq> \<tau> \<Longrightarrow> (\<sigma> \<Turnstile>\<^sub>p \<phi>) = (\<tau> \<Turnstile>\<^sub>p \<phi>)"
   (is "?sim \<sigma> \<phi> \<tau> \<Longrightarrow> ?P \<sigma> \<phi> \<tau>")
 proof (induct \<phi> arbitrary: \<sigma> \<tau>)
   fix \<sigma> \<tau>
-  show "?P \<sigma> false \<tau>" by simp
+  show "?P \<sigma> false\<^sub>p \<tau>" by simp
 next
   fix p \<sigma> \<tau>
-  assume "?sim \<sigma> (atom p) \<tau>" thus "?P \<sigma> (atom p) \<tau>"
+  assume "?sim \<sigma> (atom\<^sub>p(p)) \<tau>" thus "?P \<sigma> (atom\<^sub>p(p)) \<tau>"
     by (auto simp: seq_sim_def state_sim_def)
 next
   fix \<phi> \<psi> \<sigma> \<tau>
   assume ih: "\<And>\<sigma> \<tau>. ?sim \<sigma> \<phi> \<tau> \<Longrightarrow> ?P \<sigma> \<phi> \<tau>" 
              "\<And>\<sigma> \<tau>. ?sim \<sigma> \<psi> \<tau> \<Longrightarrow> ?P \<sigma> \<psi> \<tau>"
-     and sim: "?sim \<sigma> (implies \<phi> \<psi>) \<tau>"
+     and sim: "?sim \<sigma> (\<phi> implies\<^sub>p \<psi>) \<tau>"
   from sim have "?sim \<sigma> \<phi> \<tau>" "?sim \<sigma> \<psi> \<tau>"
     by (auto elim: seq_sim_mono)
-  with ih show "?P \<sigma> (implies \<phi> \<psi>) \<tau>" by simp
+  with ih show "?P \<sigma> (\<phi> implies\<^sub>p \<psi>) \<tau>" by simp
 next
   fix \<phi> \<sigma> \<tau>
   assume ih: "\<And>\<sigma> \<tau>. ?sim \<sigma> \<phi> \<tau> \<Longrightarrow> ?P \<sigma> \<phi> \<tau>"
-     and sim: "\<sigma> \<simeq>atoms (next \<phi>)\<simeq> \<tau>"
-  from sim have "\<sigma>[1..] \<simeq>atoms \<phi>\<simeq> \<tau>[1..]"
+     and sim: "\<sigma> \<simeq> atoms_pltl (X\<^sub>p \<phi>) \<simeq> \<tau>"
+  from sim have "(\<sigma>[1..]) \<simeq> atoms_pltl \<phi> \<simeq> (\<tau>[1..])"
     by (auto simp: seq_sim_def)
-  with ih show "?P \<sigma> (next \<phi>) \<tau>" by auto
+  with ih show "?P \<sigma> (X\<^sub>p \<phi>) \<tau>" by auto
 next
   fix \<phi> \<psi> \<sigma> \<tau>
   assume ih: "\<And>\<sigma> \<tau>. ?sim \<sigma> \<phi> \<tau> \<Longrightarrow> ?P \<sigma> \<phi> \<tau>" 
              "\<And>\<sigma> \<tau>. ?sim \<sigma> \<psi> \<tau> \<Longrightarrow> ?P \<sigma> \<psi> \<tau>"
-     and sim: "?sim \<sigma> (until \<phi> \<psi>) \<tau>"
-  from sim have "\<forall>i. \<sigma>[i..] \<simeq>atoms \<phi>\<simeq> \<tau>[i..]" "\<forall>j. \<sigma>[j..] \<simeq> atoms \<psi> \<simeq> \<tau>[j..]"
+     and sim: "?sim \<sigma> (\<phi> U\<^sub>p \<psi>) \<tau>"
+  from sim have "\<forall>i. (\<sigma>[i..]) \<simeq> atoms_pltl \<phi> \<simeq> (\<tau>[i..])" "\<forall>j. (\<sigma>[j..]) \<simeq> atoms_pltl \<psi> \<simeq> (\<tau>[j..])"
     by (auto simp: seq_sim_def state_sim_def)
   with ih have "\<forall>i. ?P (\<sigma>[i..]) \<phi> (\<tau>[i..])" "\<forall>j. ?P (\<sigma>[j..]) \<psi> (\<tau>[j..])"
     by blast+
-  thus "?P \<sigma> (until \<phi> \<psi>) \<tau>" 
+  thus "?P \<sigma> (\<phi> U\<^sub>p \<psi>) \<tau>"
     by (meson semantics_pltl.simps(5))
 qed
 
@@ -446,7 +438,7 @@ text \<open>
 
 definition characteristic_formula where
   "characteristic_formula A s \<equiv>
-   ((AND { atom p | p . p \<in> A \<and> p s }) and\<^sub>p (AND { not\<^sub>p (atom p) | p . p \<in> A \<and> \<not>(p s) }))"
+   ((AND { atom\<^sub>p(p) | p . p \<in> A \<and> p s }) and\<^sub>p (AND { not\<^sub>p (atom\<^sub>p(p)) | p . p \<in> A \<and> \<not>(p s) }))"
 
 lemma characteristic_holds: 
   "finite A \<Longrightarrow> \<sigma> \<Turnstile>\<^sub>p characteristic_formula A (\<sigma> 0)"
@@ -478,38 +470,38 @@ text \<open>
   completeness theorem: for any PLTL formula \<open>\<phi>\<close> there
   exists a next-free formula \<open>\<psi>\<close> such that the two
   formulas evaluate to the same value over stutter-free and
-  canonical sequences (w.r.t. some \<open>A \<supseteq> atoms \<phi>\<close>).
+  canonical sequences (w.r.t. some \<open>A \<supseteq> atoms_pltl \<phi>\<close>).
 \<close>
 
 lemma ex_next_free_stutter_free_canonical:
-  assumes A: "atoms \<phi> \<subseteq> A" and fin: "finite A"
-  shows "\<exists>\<psi>. next_free \<psi> \<and> atoms \<psi> \<subseteq> A \<and>
+  assumes A: "atoms_pltl \<phi> \<subseteq> A" and fin: "finite A"
+  shows "\<exists>\<psi>. next_free \<psi> \<and> atoms_pltl \<psi> \<subseteq> A \<and>
              (\<forall>\<sigma>. stutter_free \<sigma> \<and> canonical_sequence A \<sigma> \<longrightarrow> (\<sigma> \<Turnstile>\<^sub>p \<psi>) = (\<sigma> \<Turnstile>\<^sub>p \<phi>))"
     (is "\<exists>\<psi>. ?P \<phi> \<psi>")
 using A proof (induct \<phi>)
   txt \<open>The cases of \<open>false\<close> and atomic formulas are trivial.\<close>
-  have "?P false false" by auto
-  thus "\<exists>\<psi>. ?P false \<psi>" ..
+  have "?P false\<^sub>p false\<^sub>p" by auto
+  thus "\<exists>\<psi>. ?P false\<^sub>p \<psi>" ..
 next
   fix p
-  assume "atoms (atom p) \<subseteq> A"
-  hence "?P (atom p) (atom p)" by auto
-  thus "\<exists>\<psi>. ?P (atom p) \<psi>" ..
+  assume "atoms_pltl (atom\<^sub>p(p)) \<subseteq> A"
+  hence "?P (atom\<^sub>p(p)) (atom\<^sub>p(p))" by auto
+  thus "\<exists>\<psi>. ?P (atom\<^sub>p(p)) \<psi>" ..
 next
   txt \<open>Implication is easy, using the induction hypothesis.\<close>
   fix \<phi> \<psi>
-  assume "atoms \<phi> \<subseteq> A \<Longrightarrow> \<exists>\<phi>'. ?P \<phi> \<phi>'"
-     and "atoms \<psi> \<subseteq> A \<Longrightarrow> \<exists>\<psi>'. ?P \<psi> \<psi>'"
-     and "atoms (implies \<phi> \<psi>) \<subseteq> A"
+  assume "atoms_pltl \<phi> \<subseteq> A \<Longrightarrow> \<exists>\<phi>'. ?P \<phi> \<phi>'"
+     and "atoms_pltl \<psi> \<subseteq> A \<Longrightarrow> \<exists>\<psi>'. ?P \<psi> \<psi>'"
+     and "atoms_pltl (\<phi> implies\<^sub>p \<psi>) \<subseteq> A"
   then obtain \<phi>' \<psi>' where "?P \<phi> \<phi>'" "?P \<psi> \<psi>'" by auto
-  hence "?P (implies \<phi> \<psi>) (implies \<phi>' \<psi>')" by auto
-  thus "\<exists>\<chi>. ?P (implies \<phi> \<psi>) \<chi>" ..
+  hence "?P (\<phi> implies\<^sub>p \<psi>) (\<phi>' implies\<^sub>p \<psi>')" by auto
+  thus "\<exists>\<chi>. ?P (\<phi> implies\<^sub>p \<psi>) \<chi>" ..
 next
   txt \<open>The case of \<open>until\<close> follows similarly.\<close>
   fix \<phi> \<psi>
-  assume "atoms \<phi> \<subseteq> A \<Longrightarrow> \<exists>\<phi>'. ?P \<phi> \<phi>'"
-     and "atoms \<psi> \<subseteq> A \<Longrightarrow> \<exists>\<psi>'. ?P \<psi> \<psi>'"
-     and "atoms (until \<phi> \<psi>) \<subseteq> A"
+  assume "atoms_pltl \<phi> \<subseteq> A \<Longrightarrow> \<exists>\<phi>'. ?P \<phi> \<phi>'"
+     and "atoms_pltl \<psi> \<subseteq> A \<Longrightarrow> \<exists>\<psi>'. ?P \<psi> \<psi>'"
+     and "atoms_pltl (\<phi> U\<^sub>p \<psi>) \<subseteq> A"
   then obtain \<phi>' \<psi>' where 1: "?P \<phi> \<phi>'" and 2: "?P \<psi> \<psi>'" by auto
   {
     fix \<sigma>
@@ -520,31 +512,31 @@ next
     have "\<And>k. (\<sigma>[k..] \<Turnstile>\<^sub>p \<phi>') = (\<sigma>[k..] \<Turnstile>\<^sub>p \<phi>)"
      and "\<And>k. (\<sigma>[k..] \<Turnstile>\<^sub>p \<psi>') = (\<sigma>[k..] \<Turnstile>\<^sub>p \<psi>)"
       by (blast+)
-    hence "(\<sigma> \<Turnstile>\<^sub>p until \<phi>' \<psi>') = (\<sigma> \<Turnstile>\<^sub>p until \<phi> \<psi>)"
+    hence "(\<sigma> \<Turnstile>\<^sub>p \<phi>' U\<^sub>p \<psi>') = (\<sigma> \<Turnstile>\<^sub>p \<phi> U\<^sub>p \<psi>)"
       by auto
   }
-  with 1 2 have "?P (until \<phi> \<psi>) (until \<phi>' \<psi>')" by auto
-  thus "\<exists>\<chi>. ?P (until \<phi> \<psi>) \<chi>" ..
+  with 1 2 have "?P (\<phi> U\<^sub>p \<psi>) (\<phi>' U\<^sub>p \<psi>')" by auto
+  thus "\<exists>\<chi>. ?P (\<phi> U\<^sub>p \<psi>) \<chi>" ..
 next
   txt \<open>The interesting case is the one of the \<open>next\<close>-operator.\<close>
   fix \<phi>
-  assume ih: "atoms \<phi> \<subseteq> A \<Longrightarrow> \<exists>\<psi>. ?P \<phi> \<psi>" and at: "atoms (next \<phi>) \<subseteq> A"
+  assume ih: "atoms_pltl \<phi> \<subseteq> A \<Longrightarrow> \<exists>\<psi>. ?P \<phi> \<psi>" and at: "atoms_pltl (X\<^sub>p \<phi>) \<subseteq> A"
   then obtain \<psi> where psi: "?P \<phi> \<psi>" by auto
   txt \<open>A valuation (over \<open>A\<close>) is a set \<open>val \<subseteq> A\<close> of atoms. We
     define some auxiliary notions: the valuation corresponding to a state and
     the characteristic formula for a valuation. Finally, we define the formula
-    \<open>psi'\<close> that we will prove to be equivalent to \<open>next \<phi>\<close> over
+    \<open>psi'\<close> that we will prove to be equivalent to \<open>X\<^sub>p \<phi>\<close> over
     the stutter-free and canonical sequence \<open>\<sigma>\<close>.\<close>
   define stval where "stval = (\<lambda>s. { p \<in> A . p s })"
-  define chi where "chi = (\<lambda>val. ((AND {atom p | p . p \<in> val}) and\<^sub>p
-                        (AND {not\<^sub>p (atom p) | p . p \<in> A - val})))"
-  define psi' where "psi' = (Or_ltlp (\<psi> and\<^sub>p (OR {G\<^sub>p (chi val) | val . val \<subseteq> A }))
-                  (OR {(chi val) and\<^sub>p (until (chi val) ( \<psi> and\<^sub>p (chi val'))) | val val'.
+  define chi where "chi = (\<lambda>val. ((AND {atom\<^sub>p(p) | p . p \<in> val}) and\<^sub>p
+                        (AND {not\<^sub>p (atom\<^sub>p(p)) | p . p \<in> A - val})))"
+  define psi' where "psi' = ((\<psi> and\<^sub>p (OR {G\<^sub>p (chi val) | val . val \<subseteq> A })) or\<^sub>p
+                  (OR {(chi val) and\<^sub>p ((chi val) U\<^sub>p ( \<psi> and\<^sub>p (chi val'))) | val val'.
                         val \<subseteq> A \<and> val' \<subseteq> A \<and> val' \<noteq> val }))"
-        (is "_ = (Or_ltlp ( _ and\<^sub>p (OR ?ALW)) (OR ?UNT))")
+        (is "_ = (( _ and\<^sub>p (OR ?ALW)) or\<^sub>p (OR ?UNT))")
 
-  have "\<And>s. {not\<^sub>p (atom p) | p . p \<in> A - stval s}
-           = {not\<^sub>p (atom p) | p . p \<in> A \<and> \<not>(p s)}"
+  have "\<And>s. {not\<^sub>p (atom\<^sub>p(p)) | p . p \<in> A - stval s}
+           = {not\<^sub>p (atom\<^sub>p(p)) | p . p \<in> A \<and> \<not>(p s)}"
     by (auto simp: stval_def)
   hence chi1: "\<And>s. chi (stval s) = characteristic_formula A s"
     by (auto simp: chi_def stval_def characteristic_formula_def)
@@ -556,7 +548,7 @@ next
   }
   note chi2 = this
 
-  have "?UNT \<subseteq> (\<lambda>(val,val'). (chi val) and\<^sub>p (until (chi val) (\<psi> and\<^sub>p (chi val'))))
+  have "?UNT \<subseteq> (\<lambda>(val,val'). (chi val) and\<^sub>p ((chi val) U\<^sub>p (\<psi> and\<^sub>p (chi val'))))
                ` (Pow A \<times> Pow A)"
     (is "_ \<subseteq> ?S")
     by auto
@@ -571,13 +563,13 @@ next
       by (force simp: psi'_def finite_subset)
   qed
 
-  have atoms: "atoms psi' \<subseteq> A"
+  have atoms_pltl: "atoms_pltl psi' \<subseteq> A"
   proof -
-    from fin have at_chi: "\<And>val. val \<subseteq> A \<Longrightarrow> atoms (chi val) \<subseteq> A"
+    from fin have at_chi: "\<And>val. val \<subseteq> A \<Longrightarrow> atoms_pltl (chi val) \<subseteq> A"
       by (auto simp: chi_def finite_subset)
-    with fin psi have at_alw: "atoms (\<psi> and\<^sub>p (OR ?ALW)) \<subseteq> A"
+    with fin psi have at_alw: "atoms_pltl (\<psi> and\<^sub>p (OR ?ALW)) \<subseteq> A"
       by auto blast?    (** FRAGILE: auto leaves trivial goal about subset **)
-    from fin fin_UNT psi at_chi have "atoms (OR ?UNT) \<subseteq> A"
+    from fin fin_UNT psi at_chi have "atoms_pltl (OR ?UNT) \<subseteq> A"
       by auto (blast+)? (** FRAGILE: even more left-over goals here **)
     with at_alw show ?thesis by (auto simp: psi'_def)
   qed
@@ -585,7 +577,7 @@ next
   {
     fix \<sigma>
     assume st: "stutter_free \<sigma>" and can: "canonical_sequence A \<sigma>"
-    have "(\<sigma> \<Turnstile>\<^sub>p next \<phi>) = (\<sigma> \<Turnstile>\<^sub>p psi')"
+    have "(\<sigma> \<Turnstile>\<^sub>p X\<^sub>p \<phi>) = (\<sigma> \<Turnstile>\<^sub>p psi')"
     proof (cases "\<sigma> (Suc 0) = \<sigma> 0")
       case True
       txt \<open>In the case of a stuttering transition at the beginning, we must have
@@ -610,7 +602,7 @@ next
         moreover have "\<sigma> i = \<sigma> 0" by (rule alleq)
         ultimately show "(\<sigma>[n..]) i = \<sigma> i" by simp
       qed
-      with st can psi have 1: "(\<sigma> \<Turnstile>\<^sub>p next \<phi>) = (\<sigma> \<Turnstile>\<^sub>p \<psi>)" by simp
+      with st can psi have 1: "(\<sigma> \<Turnstile>\<^sub>p X\<^sub>p \<phi>) = (\<sigma> \<Turnstile>\<^sub>p \<psi>)" by simp
 
       from fin have "\<sigma> \<Turnstile>\<^sub>p chi (stval (\<sigma> 0))" by (simp add: chi1 characteristic_holds)
       with suffix have "\<sigma> \<Turnstile>\<^sub>p G\<^sub>p (chi (stval (\<sigma> 0)))" (is "_ \<Turnstile>\<^sub>p ?alw") by simp
@@ -636,7 +628,7 @@ next
 
     next
       case False
-      txt \<open>Otherwise, \<open>\<sigma> \<Turnstile>\<^sub>p next \<phi>\<close> is equivalent to \<open>\<sigma>\<close> satisfying
+      txt \<open>Otherwise, \<open>\<sigma> \<Turnstile>\<^sub>p X\<^sub>p \<phi>\<close> is equivalent to \<open>\<sigma>\<close> satisfying
         the second disjunct of \<open>psi'\<close>. We show both implications separately.\<close>
       let ?val = "stval (\<sigma> 0)"
       let ?val' = "stval (\<sigma> 1)"
@@ -645,7 +637,7 @@ next
         
       show ?thesis
       proof
-        assume phi: "\<sigma> \<Turnstile>\<^sub>p next \<phi>"
+        assume phi: "\<sigma> \<Turnstile>\<^sub>p X\<^sub>p \<phi>"
         from fin have 1: "\<sigma> \<Turnstile>\<^sub>p chi ?val" by (simp add: chi1 characteristic_holds)
 
         from st can have "stutter_free (\<sigma>[1..])" "canonical_sequence A (\<sigma>[1..])"
@@ -656,7 +648,7 @@ next
           by (rule characteristic_holds)
         hence 3: "\<sigma>[1..] \<Turnstile>\<^sub>p chi ?val'" by (simp add: chi1)
 
-        from 1 2 3 have "\<sigma> \<Turnstile>\<^sub>p And_ltlp (chi ?val) (until (chi ?val) (And_ltlp \<psi> (chi ?val')))"
+        from 1 2 3 have "\<sigma> \<Turnstile>\<^sub>p And_ltlp (chi ?val) ((chi ?val) U\<^sub>p (And_ltlp \<psi> (chi ?val')))"
           (is "_ \<Turnstile>\<^sub>p ?unt")
           by auto
         moreover from vals have "?unt \<in> ?UNT"
@@ -670,7 +662,7 @@ next
         have "\<not>(\<sigma> \<Turnstile>\<^sub>p OR ?ALW)"
         proof
           assume "\<sigma> \<Turnstile>\<^sub>p OR ?ALW"
-          with fin obtain val where 1: "val \<subseteq> A" and 2: "\<forall>n. \<sigma>[n..] \<Turnstile>\<^sub>p chi val"
+          with fin obtain val where 1: "val \<subseteq> A" and 2: "\<forall>n. (\<sigma>[n..] \<Turnstile>\<^sub>p chi val)"
             by (force simp: finite_subset)
           from 2 have "\<sigma>[0..] \<Turnstile>\<^sub>p chi val" ..
           with 1 have "val = ?val" by (simp add: chi2)
@@ -685,7 +677,7 @@ next
           val: "val \<subseteq> A" "val' \<subseteq> A" "val' \<noteq> val" and
           now: "\<sigma> \<Turnstile>\<^sub>p chi val" and
           k: "\<sigma>[k..] \<Turnstile>\<^sub>p \<psi>" "\<sigma>[k..] \<Turnstile>\<^sub>p chi val'" and
-          i: "\<forall>i<k. \<sigma>[i..] \<Turnstile>\<^sub>p chi val"
+          i: "\<forall>i<k. (\<sigma>[i..] \<Turnstile>\<^sub>p chi val)"
           by auto (blast+)?  (* FRAGILE: similar as above *)
 
         from val now have 1: "val = ?val" by (simp add: chi2)
@@ -714,21 +706,21 @@ next
         moreover
         from st can have "stutter_free (\<sigma>[1..])" "canonical_sequence A (\<sigma>[1..])"
           by (auto simp: stutter_free_suffix canonical_suffix)
-        ultimately show "\<sigma> \<Turnstile>\<^sub>p next \<phi>" using \<open>\<sigma>[k..] \<Turnstile>\<^sub>p \<psi>\<close> psi by auto
+        ultimately show "\<sigma> \<Turnstile>\<^sub>p X\<^sub>p \<phi>" using \<open>\<sigma>[k..] \<Turnstile>\<^sub>p \<psi>\<close> psi by auto
       qed
     qed
   }
-  with nf atoms show "\<exists>\<psi>'. ?P (next \<phi>) \<psi>'" by blast
+  with nf atoms_pltl show "\<exists>\<psi>'. ?P (X\<^sub>p \<phi>) \<psi>'" by blast
 qed
 
 text \<open>
   Comparing the definition of the next-free formula in the case of
-  formulas \<open>next \<phi>\<close> with the one that appears in~\cite{peled:ltl-x},
+  formulas \<open>X\<^sub>p \<phi>\<close> with the one that appears in~\cite{peled:ltl-x},
   there is a subtle difference. Peled and Wilke define the second disjunct as
   a disjunction of formulas
 %
   \begin{center}\(
-    \<open>until (chi val) (and \<psi> (chi val'))\<close>
+    \<open>(chi val) U\<^sub>p (\<psi> and\<^sub>p (chi val'))\<close>
   \)\end{center}
 %
   for subsets \<open>val, val' \<subseteq> A\<close> whereas we conjoin the formula
@@ -744,26 +736,26 @@ text \<open>
   formal proofs.
 
   We now show that any stuttering invariant PLTL formula
-  can be expressed without the \<open>next\<close> operator.
+  can be expressed without the \<open>X\<^sub>p\<close> operator.
 \<close>
 
 theorem stutter_invariant_next_free:
   assumes phi: "stutter_invariant \<phi>"
-  obtains \<psi> where "next_free \<psi>" "atoms \<psi> \<subseteq> atoms \<phi>"
+  obtains \<psi> where "next_free \<psi>" "atoms_pltl \<psi> \<subseteq> atoms_pltl \<phi>"
                   "\<forall>\<sigma>. (\<sigma> \<Turnstile>\<^sub>p \<psi>) = (\<sigma> \<Turnstile>\<^sub>p \<phi>)"
 proof -
-  have "atoms \<phi> \<subseteq> atoms \<phi>" "finite (atoms \<phi>)" by simp_all
+  have "atoms_pltl \<phi> \<subseteq> atoms_pltl \<phi>" "finite (atoms_pltl \<phi>)" by simp_all
   then obtain \<psi> where
-    psi: "next_free \<psi>" "atoms \<psi> \<subseteq> atoms \<phi>" and
-    equiv: "\<forall>\<sigma>. stutter_free \<sigma> \<and> canonical_sequence (atoms \<phi>) \<sigma> \<longrightarrow> (\<sigma> \<Turnstile>\<^sub>p \<psi>) = (\<sigma> \<Turnstile>\<^sub>p \<phi>)"
+    psi: "next_free \<psi>" "atoms_pltl \<psi> \<subseteq> atoms_pltl \<phi>" and
+    equiv: "\<forall>\<sigma>. stutter_free \<sigma> \<and> canonical_sequence (atoms_pltl \<phi>) \<sigma> \<longrightarrow> (\<sigma> \<Turnstile>\<^sub>p \<psi>) = (\<sigma> \<Turnstile>\<^sub>p \<phi>)"
     by (blast dest: ex_next_free_stutter_free_canonical)
   from \<open>next_free \<psi>\<close> have sinv: "stutter_invariant \<psi>"
     by (rule next_free_stutter_invariant)
   {
     fix \<sigma>
-    obtain \<tau> where 1: "\<tau> \<simeq> atoms \<phi> \<simeq> \<sigma>" and 2: "canonical_sequence (atoms \<phi>) \<tau>"
+    obtain \<tau> where 1: "\<tau> \<simeq> atoms_pltl \<phi> \<simeq> \<sigma>" and 2: "canonical_sequence (atoms_pltl \<phi>) \<tau>"
       by (rule canonical_exists)
-    from 1 \<open>atoms \<psi> \<subseteq> atoms \<phi>\<close> have 3: "\<tau> \<simeq> atoms \<psi> \<simeq> \<sigma>"
+    from 1 \<open>atoms_pltl \<psi> \<subseteq> atoms_pltl \<phi>\<close> have 3: "\<tau> \<simeq> atoms_pltl \<psi> \<simeq> \<sigma>"
       by (rule seq_sim_mono)
 
     from 1 have "(\<sigma> \<Turnstile>\<^sub>p \<phi>) = (\<tau> \<Turnstile>\<^sub>p \<phi>)" by (simp add: pltl_seq_sim)
@@ -786,11 +778,11 @@ text \<open>
 
 theorem pltl_stutter_invariant:
   "stutter_invariant \<phi> \<longleftrightarrow> 
-   (\<exists>\<psi>. next_free \<psi> \<and> atoms \<psi> \<subseteq> atoms \<phi> \<and> (\<forall>\<sigma>. \<sigma> \<Turnstile>\<^sub>p \<psi> \<longleftrightarrow> \<sigma> \<Turnstile>\<^sub>p \<phi>))"
+   (\<exists>\<psi>. next_free \<psi> \<and> atoms_pltl \<psi> \<subseteq> atoms_pltl \<phi> \<and> (\<forall>\<sigma>. \<sigma> \<Turnstile>\<^sub>p \<psi> \<longleftrightarrow> \<sigma> \<Turnstile>\<^sub>p \<phi>))"
 proof -
   {
     assume "stutter_invariant \<phi>"
-    hence "\<exists>\<psi>. next_free \<psi> \<and> atoms \<psi> \<subseteq> atoms \<phi> \<and> (\<forall>\<sigma>. \<sigma> \<Turnstile>\<^sub>p \<psi> \<longleftrightarrow> \<sigma> \<Turnstile>\<^sub>p \<phi>)"
+    hence "\<exists>\<psi>. next_free \<psi> \<and> atoms_pltl \<psi> \<subseteq> atoms_pltl \<phi> \<and> (\<forall>\<sigma>. \<sigma> \<Turnstile>\<^sub>p \<psi> \<longleftrightarrow> \<sigma> \<Turnstile>\<^sub>p \<phi>)"
       by (rule stutter_invariant_next_free) blast
   }
   moreover
@@ -801,6 +793,52 @@ proof -
     with 2 have "stutter_invariant \<phi>" by blast
   }
   ultimately show ?thesis by blast
+qed
+
+
+subsection \<open>Stutter Invariance for LTL with Syntactic Sugar\<close>
+
+text \<open>We lift the results for PLTL to an extensive version of LTL.\<close>
+
+primrec ltlc_next_free :: "'a ltlc \<Rightarrow> bool"
+  where
+    "ltlc_next_free true\<^sub>c = True"
+  | "ltlc_next_free false\<^sub>c = True"
+  | "ltlc_next_free (prop\<^sub>c(q)) = True"
+  | "ltlc_next_free (not\<^sub>c \<phi>) = ltlc_next_free \<phi>"
+  | "ltlc_next_free (\<phi> and\<^sub>c \<psi>) = (ltlc_next_free \<phi> \<and> ltlc_next_free \<psi>)"
+  | "ltlc_next_free (\<phi> or\<^sub>c \<psi>) = (ltlc_next_free \<phi> \<and> ltlc_next_free \<psi>)"
+  | "ltlc_next_free (\<phi> implies\<^sub>c \<psi>) = (ltlc_next_free \<phi> \<and> ltlc_next_free \<psi>)"
+  | "ltlc_next_free (X\<^sub>c \<phi>) = False"
+  | "ltlc_next_free (F\<^sub>c \<phi>) = ltlc_next_free \<phi>"
+  | "ltlc_next_free (G\<^sub>c \<phi>) = ltlc_next_free \<phi>"
+  | "ltlc_next_free (\<phi> U\<^sub>c \<psi>) = (ltlc_next_free \<phi> \<and> ltlc_next_free \<psi>)"
+  | "ltlc_next_free (\<phi> R\<^sub>c \<psi>) = (ltlc_next_free \<phi> \<and> ltlc_next_free \<psi>)"
+  | "ltlc_next_free (\<phi> W\<^sub>c \<psi>) = (ltlc_next_free \<phi> \<and> ltlc_next_free \<psi>)"
+  | "ltlc_next_free (\<phi> M\<^sub>c \<psi>) = (ltlc_next_free \<phi> \<and> ltlc_next_free \<psi>)"
+
+lemma ltlc_next_free_iff[simp]: "next_free (ltlc_to_pltl \<phi>) \<longleftrightarrow> ltlc_next_free \<phi>"
+  by (induction \<phi>) auto
+
+text \<open>A next free formula cannot distinguish between stutter-equivalent runs.\<close>
+
+theorem ltlc_next_free_stutter_invariant:
+  assumes next_free: "ltlc_next_free \<phi>"
+  assumes eq: "r \<approx> r'"
+  shows "r \<Turnstile>\<^sub>c \<phi> \<longleftrightarrow> r' \<Turnstile>\<^sub>c \<phi>"
+proof -
+  {
+    fix r r'
+    assume eq: "r \<approx> r'" and holds: "r \<Turnstile>\<^sub>c \<phi>"
+    then have "r \<Turnstile>\<^sub>p (ltlc_to_pltl \<phi>)"by simp
+
+    from next_free_stutter_invariant[of "ltlc_to_pltl \<phi>"] next_free
+    have "PLTL.stutter_invariant (ltlc_to_pltl \<phi>)" by simp
+    from stutter_invariantD[OF this eq] holds have "r' \<Turnstile>\<^sub>c \<phi>" by simp
+  } note aux=this
+
+  from aux[of r r'] aux[of r' r] eq stutter_equiv_sym[OF eq] show ?thesis
+    by blast
 qed
 
 
